tweaks to st2

lib/st2.fst
@@ -5,6 +5,13 @@ assume val v1 : a:Type -> a -> Tot a
 type heap2 = heap * heap
 
 kind STWP (a:Type) = (a -> heap -> Type) -> heap -> Type
+
+type comp (a:Type) (b:Type) (wp0:STWP a) (wp1:STWP b) (p:((a * b) -> heap2 -> Type)) (h2:heap2) =
+    wp0 (fun y0 h0 ->
+      wp1 (fun y1 h1 -> p (y0, y1) (h0, h1))
+      (snd h2))
+    (fst h2)
+
 assume val compose2: a0:Type -> b0:Type -> wp0:(a0 -> STWP b0) -> wlp0:(a0 -> STWP b0)
                   -> a1:Type -> b1:Type -> wp1:(a1 -> STWP b1) -> wlp1:(a1 -> STWP b1)
                   -> =c0:(x0:a0 -> STATE b0 (wp0 x0) (wlp0 x0))
@@ -12,16 +19,8 @@ assume val compose2: a0:Type -> b0:Type -> wp0:(a0 -> STWP b0) -> wlp0:(a0 -> ST
                   -> x0:a0
                   -> x1:a1
                   -> ST2Core (b0 * b1)
-                            (fun 'p (h2:heap2) ->
-                                  wp0 x0 (fun y0 h0 ->
-                                    wp1 x1 (fun y1 h1 -> 'p (y0, y1) (h0, h1))
-                                           (snd h2))
-                                           (fst h2))
-                            (fun 'p (h2:heap2) ->
-                                   wlp0 x0 (fun y0 h0 ->
-                                     wlp1 x1 (fun y1 h1 -> 'p (y0, y1) (h0, h1))
-                                            (snd h2))
-                                            (fst h2))
+                             (comp b0 b1 (wp0 x0) (wp1 x1))
+                             (comp b0 b1 (wlp0 x0) (wlp1 x1))
 
 module Sample
 open ST2
@@ -30,9 +29,9 @@ open Heap
 let f x = x := !x - !x
 let g x = x := 0
 
-val equiv: x:ref int
-        -> y:ref int
-        -> ST2 (unit * unit)
-               (fun _ -> True) //x, y may be high-references
-               (fun _ _ h2' -> sel (fst h2') x == sel (snd h2') x) //their contents are equal afterwards
-let equiv x y = compose2 f g x y
+val equiv1: x:ref int
+         -> y:ref int
+         -> ST2 (unit * unit)
+                (fun _ -> True) //x, y may be high-references
+                (fun _ _ h2' -> sel (fst h2') x == sel (snd h2') y) //their contents are equal afterwards
+let equiv1 x y = compose2 f g x y
